src/trans/SplitAcqCommon.v
@@ -1,200 +1,92 @@
 From sflib Require Import sflib.
 From Paco Require Import paco.
 
+From PromisingLib Require Import Axioms.
 From PromisingLib Require Import Basic.
 From PromisingLib Require Import Loc.
+From PromisingLib Require Import DataStructure.
+From PromisingLib Require Import DenseOrder.
 From PromisingLib Require Import Language.
-
 From PromisingLib Require Import Event.
+
 Require Import Time.
 Require Import View.
+Require Import BoolMap.
+Require Import Promises.
 Require Import Cell.
 Require Import Memory.
+Require Import Global.
 Require Import TView.
 Require Import Local.
 Require Import Thread.
 Require Import Configuration.
 
-Require Import FulfillStep.
-
-Require Import SimMemory.
-Require Import SimPromises.
 Require Import SimLocal.
-Require Import SimThread.
+Require Import SimMemory.
+Require Import SimGlobal.
 
 Set Implicit Arguments.
 
 
 Definition local_acquired (lc:Local.t) :=
-  (Local.mk (TView.read_fence_tview (Local.tview lc) Ordering.acqrel) (Local.promises lc)).
+  (Local.mk
+     (TView.read_fence_tview (Local.tview lc) Ordering.acqrel)
+     (Local.promises lc)
+     (Local.reserves lc)).
 
-Lemma sim_local_promise_acquired
-      lc1_src mem1_src
-      lc1_tgt mem1_tgt
-      lc2_tgt mem2_tgt
-      loc from to msg kind
-      (STEP_TGT: Local.promise_step lc1_tgt mem1_tgt loc from to msg lc2_tgt mem2_tgt kind)
-      (LOCAL1: sim_local SimPromises.bot lc1_src (local_acquired lc1_tgt))
-      (MEM1: sim_memory mem1_src mem1_tgt)
-      (WF1_SRC: Local.wf lc1_src mem1_src)
-      (WF1_TGT: Local.wf lc1_tgt mem1_tgt)
-      (MEM1_SRC: Memory.closed mem1_src)
-      (MEM1_TGT: Memory.closed mem1_tgt):
-  exists lc2_src mem2_src,
-    <<STEP_SRC: Local.promise_step lc1_src mem1_src loc from to msg lc2_src mem2_src kind>> /\
-    <<LOCAL2: sim_local SimPromises.bot lc2_src (local_acquired lc2_tgt)>> /\
-    <<MEM2: sim_memory mem2_src mem2_tgt>>.
+Lemma local_acquired_wf
+      lc gl
+      (WF: Local.wf lc gl):
+  Local.wf (local_acquired lc) gl.
 Proof.
-  inv LOCAL1. inv STEP_TGT.
-  exploit SimPromises.promise_bot; eauto.
-  { apply WF1_SRC. }
-  { apply WF1_TGT. }
-  i. des.
-  exploit Memory.promise_future; try apply PROMISE_SRC; try apply WF1_SRC; eauto.
-  { destruct msg; ss. inv CLOSED. econs.
-    eapply sim_memory_closed_opt_view; eauto. }
-  i. des.
-  esplits; eauto.
-  - econs; eauto.
-    destruct msg; ss. inv CLOSED. econs.
-    eapply sim_memory_closed_opt_view; eauto.
-  - econs; eauto.
+  inv WF. econs; ss.
+  - inv TVIEW_WF. econs; ss.
+    + condtac; ss. etrans; eauto.
+    + condtac; ss. refl.
+  - inv TVIEW_CLOSED. econs; ss.
 Qed.
 
-Lemma sim_local_fulfill_acquired
-      lc1_src sc1_src mem1_src
-      lc1_tgt sc1_tgt mem1_tgt
-      lc2_tgt sc2_tgt
-      loc from to val releasedm_src releasedm_tgt released ord_src ord_tgt
-      (RELM_LE: View.opt_le releasedm_src releasedm_tgt)
-      (RELM_WF: View.opt_wf releasedm_src)
-      (RELM_CLOSED: Memory.closed_opt_view releasedm_src mem1_src)
-      (RELM_TGT: Time.le (View.rlx (View.unwrap releasedm_tgt) loc) from)
-      (WF_RELM_TGT: View.opt_wf releasedm_tgt)
-      (ORD: Ordering.le ord_src ord_tgt)
-      (ORD_TGT: Ordering.le ord_tgt Ordering.strong_relaxed)
-      (STEP_TGT: fulfill_step lc1_tgt sc1_tgt loc from to val releasedm_tgt released ord_tgt lc2_tgt sc2_tgt)
-      (LOCAL1: sim_local SimPromises.bot lc1_src (local_acquired lc1_tgt))
-      (ACQUIRED1: View.le (TView.cur (Local.tview lc1_src))
-                          (View.join (TView.cur (Local.tview lc1_tgt)) (View.unwrap releasedm_tgt)))
-      (SC1: TimeMap.le sc1_src sc1_tgt)
-      (MEM1: sim_memory mem1_src mem1_tgt)
-      (WF1_SRC: Local.wf lc1_src mem1_src)
-      (WF1_TGT: Local.wf lc1_tgt mem1_tgt)
-      (SC1_SRC: Memory.closed_timemap sc1_src mem1_src)
-      (SC1_TGT: Memory.closed_timemap sc1_tgt mem1_tgt)
-      (MEM1_SRC: Memory.closed mem1_src)
-      (MEM1_TGT: Memory.closed mem1_tgt):
-  exists lc2_src sc2_src,
-    <<STEP_SRC: fulfill_step lc1_src sc1_src loc from to val releasedm_src released ord_src lc2_src sc2_src>> /\
-    <<LOCAL2: sim_local SimPromises.bot lc2_src (local_acquired lc2_tgt)>> /\
-    <<SC2: TimeMap.le sc2_src sc2_tgt>>.
+Lemma sim_local_internal_acquired
+      lc1_src gl1_src
+      lc1_tgt gl1_tgt
+      e lc2_tgt gl2_tgt
+      (STEP_TGT: Local.internal_step e lc1_tgt gl1_tgt lc2_tgt gl2_tgt)
+      (LOCAL1: sim_local lc1_src (local_acquired lc1_tgt))
+      (GLOBAL1: sim_global gl1_src gl1_tgt)
+      (LC_WF1_SRC: Local.wf lc1_src gl1_src)
+      (LC_WF1_TGT: Local.wf lc1_tgt gl1_tgt)
+      (GL_WF1_SRC: Global.wf gl1_src)
+      (GL_WF1_TGT: Global.wf gl1_tgt):
+  exists lc2_src gl2_src,
+    <<STEP_SRC: Local.internal_step e lc1_src gl1_src lc2_src gl2_src>> /\
+    <<LOCAL2: sim_local lc2_src (local_acquired lc2_tgt)>> /\
+    <<GLOBAL2: sim_global gl2_src gl2_tgt>>.
 Proof.
-  inv STEP_TGT.
-  assert (RELT_LE:
-   View.opt_le
-     (TView.write_released (Local.tview lc1_src) sc1_src loc to releasedm_src ord_src)
-     (TView.write_released (Local.tview lc1_tgt) sc2_tgt loc to releasedm_tgt ord_tgt)).
-  { unfold TView.write_released, TView.write_tview. ss. viewtac.
-    repeat (condtac; aggrtac;
-            try match goal with
-                | [|- View.opt_le _ _] => econs
-                end);
-      try apply WF1_TGT.
-    - etrans; eauto. aggrtac.
-    - etrans; [apply WF1_SRC|]. etrans; eauto. aggrtac.
-    - etrans; [apply LOCAL1|]. aggrtac.
-  }
-  assert (RELT_WF:
-   View.opt_wf (TView.write_released (Local.tview lc1_src) sc1_src loc to releasedm_src ord_src)).
-  { unfold TView.write_released. condtac; econs.
-    repeat (try condtac; viewtac; try apply WF1_SRC).
-  }
-  exploit SimPromises.remove_bot; try exact REMOVE;
-    try exact MEM1; try apply LOCAL1; eauto.
-  i. des. esplits.
-  - econs; eauto.
-    inv WRITABLE. econs.
-    eapply TimeFacts.le_lt_lt; [apply ACQUIRED1|]. viewtac.
-    eapply TimeFacts.le_lt_lt; eauto.
-  - econs; eauto. s. unfold TView.write_tview, TView.read_fence_tview. ss.
-    econs; ss; repeat (try condtac; aggrtac).
-    all: try by destruct ord_src, ord_tgt.
-    all: try by apply WF1_TGT.
-    + etrans; [apply LOCAL1|]. aggrtac.
-    + etrans; [apply LOCAL1|]. aggrtac.
-    + etrans; [apply WF1_SRC|]. etrans; [apply LOCAL1|]. aggrtac.
-    + etrans; [apply LOCAL1|]. aggrtac.
-  - ss.
-Qed.
-
-Lemma sim_local_write_acquired
-      lc1_src sc1_src mem1_src
-      lc1_tgt sc1_tgt mem1_tgt
-      lc2_tgt sc2_tgt mem2_tgt
-      loc from to val releasedm_src releasedm_tgt released_tgt ord_src ord_tgt kind
-      (RELM_LE: View.opt_le releasedm_src releasedm_tgt)
-      (RELM_SRC_WF: View.opt_wf releasedm_src)
-      (RELM_SRC_CLOSED: Memory.closed_opt_view releasedm_src mem1_src)
-      (RELM_TGT_WF: View.opt_wf releasedm_tgt)
-      (RELM_TGT_CLOSED: Memory.closed_opt_view releasedm_tgt mem1_tgt)
-      (RELM_TGT: Time.le (View.rlx (View.unwrap releasedm_tgt) loc) from)
-      (ORD: Ordering.le ord_src ord_tgt)
-      (ORD_TGT: Ordering.le ord_tgt Ordering.strong_relaxed)
-      (STEP_TGT: Local.write_step lc1_tgt sc1_tgt mem1_tgt loc from to val releasedm_tgt released_tgt ord_tgt lc2_tgt sc2_tgt mem2_tgt kind)
-      (LOCAL1: sim_local SimPromises.bot lc1_src (local_acquired lc1_tgt))
-      (ACQUIRED1: View.le (TView.cur (Local.tview lc1_src))
-                          (View.join (TView.cur (Local.tview lc1_tgt)) (View.unwrap releasedm_tgt)))
-      (SC1: TimeMap.le sc1_src sc1_tgt)
-      (MEM1: sim_memory mem1_src mem1_tgt)
-      (WF1_SRC: Local.wf lc1_src mem1_src)
-      (WF1_TGT: Local.wf lc1_tgt mem1_tgt)
-      (SC1_SRC: Memory.closed_timemap sc1_src mem1_src)
-      (SC1_TGT: Memory.closed_timemap sc1_tgt mem1_tgt)
-      (MEM1_SRC: Memory.closed mem1_src)
-      (MEM1_TGT: Memory.closed mem1_tgt):
-  exists released_src lc2_src sc2_src mem2_src,
-    <<STEP_SRC: Local.write_step lc1_src sc1_src mem1_src loc from to val releasedm_src released_src ord_src lc2_src sc2_src mem2_src kind>> /\
-    <<REL2: View.opt_le released_src released_tgt>> /\
-    <<LOCAL2: sim_local SimPromises.bot lc2_src (local_acquired lc2_tgt)>> /\
-    <<SC2: TimeMap.le sc2_src sc2_tgt>> /\
-    <<MEM2: sim_memory mem2_src mem2_tgt>>.
-Proof.
-  exploit write_promise_fulfill; eauto. i. des.
-  exploit Local.promise_step_future; eauto. i. des.
-  exploit sim_local_promise_acquired; eauto. i. des.
-  exploit Local.promise_step_future; eauto. i. des.
-  hexploit sim_local_fulfill_acquired; try apply STEP2;
-    try apply LOCAL2; try apply MEM2; eauto.
-  { eapply Memory.future_closed_opt_view; eauto. }
-  { inv STEP_SRC. inv STEP1. ss. }
-  i. des.
-  exploit promise_fulfill_write_sim_memory; try exact STEP_SRC; try exact STEP_SRC0; eauto.
-  { i. hexploit ORD0; eauto.
-    i. des. splits; auto. eapply sim_local_nonsynch_loc; eauto.
-  }
-  i. des. esplits; eauto. etrans; eauto.
+  exploit local_acquired_wf; try exact LC_WF1_TGT. i.
+  exploit sim_local_internal; try exact LOCAL1; eauto.
+  unfold local_acquired. destruct lc1_tgt.
+  inv STEP_TGT; inv LOCAL; ss; eauto.
 Qed.
 
 Lemma sim_local_read_acquired
-      lc1_src mem1_src
-      lc1_tgt mem1_tgt
+      lc1_src gl1_src
+      lc1_tgt gl1_tgt
       lc2_tgt
       loc ts val released_tgt
-      (STEP_TGT: Local.read_step lc1_tgt mem1_tgt loc ts val released_tgt Ordering.relaxed lc2_tgt)
-      (LOCAL1: sim_local SimPromises.bot lc1_src lc1_tgt)
-      (MEM1: sim_memory mem1_src mem1_tgt)
-      (WF1_SRC: Local.wf lc1_src mem1_src)
-      (WF1_TGT: Local.wf lc1_tgt mem1_tgt)
-      (MEM1_SRC: Memory.closed mem1_src)
-      (MEM1_TGT: Memory.closed mem1_tgt):
+      (STEP_TGT: Local.read_step lc1_tgt gl1_tgt loc ts val released_tgt Ordering.relaxed lc2_tgt)
+      (LOCAL1: sim_local lc1_src lc1_tgt)
+      (GLOBAL1: sim_global gl1_src gl1_tgt)
+      (LC_WF1_SRC: Local.wf lc1_src gl1_src)
+      (LC_WF1_TGT: Local.wf lc1_tgt gl1_tgt)
+      (GL_WF1_SRC: Global.wf gl1_src)
+      (GL_WF1_TGT: Global.wf gl1_tgt):
   exists released_src lc2_src,
     <<REL: View.opt_le released_src released_tgt>> /\
-    <<STEP_SRC: Local.read_step lc1_src mem1_src loc ts val released_src Ordering.acqrel lc2_src>> /\
-    <<LOCAL2: sim_local SimPromises.bot lc2_src (local_acquired lc2_tgt)>>.
+    <<STEP_SRC: Local.read_step lc1_src gl1_src loc ts val released_src Ordering.acqrel lc2_src>> /\
+    <<LOCAL2: sim_local lc2_src (local_acquired lc2_tgt)>>.
 Proof.
   inv LOCAL1. inv STEP_TGT.
-  exploit sim_memory_get; try apply GET; try apply MEM1. i. des. inv MSG.
+  exploit sim_memory_get; try apply GET; try apply GLOBAL1. i. des. inv MSG.
   esplits; eauto.
   - econs; eauto; try by (etrans; eauto). inv READABLE. econs; ss; i.
     + rewrite <- PLN. apply TVIEW.
@@ -203,68 +95,166 @@ Proof.
     unfold TView.read_tview, TView.read_fence_tview. ss.
     econs; repeat (condtac; aggrtac).
     all: try by apply TVIEW.
-    all: try by apply WF1_TGT.
-    + rewrite <- ? View.join_l. etrans; [apply TVIEW|]. apply WF1_TGT.
-    + inv MEM1_TGT. exploit CLOSED; eauto. i. des.
+    all: try by apply LC_WF1_TGT.
+    + rewrite <- ? View.join_l. etrans; [apply TVIEW|]. apply LC_WF1_TGT.
+    + inv GL_WF1_TGT. inv MEM_CLOSED.
+      exploit CLOSED; eauto. i. des.
       apply View.unwrap_opt_wf. inv MSG_WF. ss.
     + rewrite <- ? View.join_l. apply TVIEW.
-    + inv MEM1_TGT. exploit CLOSED; eauto. i. des.
+    + inv GL_WF1_TGT. inv MEM_CLOSED.
+      exploit CLOSED; eauto. i. des.
       apply View.unwrap_opt_wf. inv MSG_WF. ss.
+Qed.
+
+Lemma sim_local_write_acquired
+      lc1_src gl1_src
+      lc1_tgt gl1_tgt
+      lc2_tgt gl2_tgt
+      loc from to val releasedm_src releasedm_tgt released_tgt ord_src ord_tgt
+      (RELM_LE: View.opt_le releasedm_src releasedm_tgt)
+      (RELM_WF_SRC: View.opt_wf releasedm_src)
+      (RELM_CLOSED_SRC: Memory.closed_opt_view releasedm_src (Global.memory gl1_src))
+      (RELM_WF_TGT: View.opt_wf releasedm_tgt)
+      (RELM_TO_TGT: Time.le (View.rlx (View.unwrap releasedm_tgt) loc) from)
+      (ORD: Ordering.le ord_src ord_tgt)
+      (ORD_TGT: Ordering.le ord_tgt Ordering.strong_relaxed)
+      (STEP_TGT: Local.write_step lc1_tgt gl1_tgt loc from to val releasedm_tgt released_tgt ord_tgt lc2_tgt gl2_tgt)
+      (LOCAL1: sim_local lc1_src (local_acquired lc1_tgt))
+      (GLOBAL1: sim_global gl1_src gl1_tgt)
+      (LC_WF1_SRC: Local.wf lc1_src gl1_src)
+      (LC_WF1_TGT: Local.wf lc1_tgt gl1_tgt)
+      (GL_WF1_SRC: Global.wf gl1_src)
+      (GL_WF1_TGT: Global.wf gl1_tgt)
+      (ACQUIRED1: View.le (TView.cur (Local.tview lc1_src))
+                          (View.join (TView.cur (Local.tview lc1_tgt)) (View.unwrap releasedm_tgt))):
+  exists released_src lc2_src gl2_src,
+    <<STEP_SRC: Local.write_step lc1_src gl1_src loc from to val releasedm_src released_src ord_src lc2_src gl2_src>> /\
+    <<REL: View.opt_le released_src released_tgt>> /\
+    <<LOCAL2: sim_local lc2_src (local_acquired lc2_tgt)>> /\
+    <<GLOBAL2: sim_global gl2_src gl2_tgt>>.
+Proof.
+  inv STEP_TGT.
+  assert (REL:
+   View.opt_le
+     (TView.write_released (Local.tview lc1_src) loc to releasedm_src ord_src)
+     (TView.write_released (Local.tview lc1_tgt) loc to releasedm_tgt ord_tgt)).
+  { unfold TView.write_released, TView.write_tview. ss. viewtac.
+    repeat (condtac; aggrtac;
+            try match goal with
+                | [|- View.opt_le _ _] => econs
+                end);
+      try apply LC_WF1_TGT.
+    - etrans; eauto. aggrtac.
+    - etrans; [apply LC_WF1_SRC|]. etrans; eauto. aggrtac.
+    - etrans; [apply LOCAL1|]. aggrtac.
+  }
+  assert (REL_WF:
+   View.opt_wf (TView.write_released (Local.tview lc1_src) loc to releasedm_src ord_src)).
+  { unfold TView.write_released. condtac; econs.
+    repeat (try condtac; viewtac; try apply LC_WF1_SRC).
+  }
+  exploit sim_memory_add_exists; try exact WRITE; try apply GLOBAL1.
+  { econs 1. exact REL_WF. }
+  { econs; try exact REL; try refl.
+    apply ord_implb. eassumption.
+  }
+  i. des.
+  exploit sim_local_fulfill; try apply LOCAL1; try exact ORD; eauto. i.
+  esplits.
+  - econs; eauto.
+    inv WRITABLE. econs.
+    eapply TimeFacts.le_lt_lt; [apply ACQUIRED1|]. viewtac.
+    eapply TimeFacts.le_lt_lt; eauto.
+    exploit Memory.add_ts; eauto.
+  - ss.
+  - inv LOCAL1. ss. econs; ss.
+    unfold TView.write_tview, TView.read_fence_tview. ss.
+    econs; ss; repeat (try condtac; aggrtac).
+    all: try by destruct ord_src, ord_tgt.
+    all: try by apply LC_WF1_TGT.
+    + etrans; [apply TVIEW|]. aggrtac.
+    + etrans; [apply TVIEW|]. aggrtac.
+    + etrans; [apply LC_WF1_SRC|].
+      etrans; [apply TVIEW|]. aggrtac.
+    + etrans; [apply TVIEW|]. aggrtac.
+  - econs; ss. apply GLOBAL1.
+Qed.
+
+Lemma sim_local_update_acquired
+      lc1_src gl1_src
+      lc1_tgt gl1_tgt
+      lc2_tgt
+      lc3_tgt gl3_tgt
+      loc ts1 val1 released1_tgt
+      to2 val2 released2_tgt ord2_src ord2_tgt
+      (STEP1_TGT: Local.read_step lc1_tgt gl1_tgt loc ts1 val1 released1_tgt Ordering.relaxed lc2_tgt)
+      (STEP2_TGT: Local.write_step lc2_tgt gl1_tgt loc ts1 to2 val2 released1_tgt released2_tgt ord2_tgt lc3_tgt gl3_tgt)
+      (ORD2: Ordering.le ord2_src ord2_tgt)
+      (ORD2_TGT: Ordering.le ord2_tgt Ordering.strong_relaxed)
+      (LOCAL1: sim_local lc1_src lc1_tgt)
+      (GLOBAL1: sim_global gl1_src gl1_tgt)
+      (LC_WF1_SRC: Local.wf lc1_src gl1_src)
+      (LC_WF1_TGT: Local.wf lc1_tgt gl1_tgt)
+      (GL_WF1_SRC: Global.wf gl1_src)
+      (GL_WF1_TGT: Global.wf gl1_tgt):
+  exists released1_src released2_src lc2_src lc3_src gl3_src,
+    <<REL1: View.opt_le released1_src released1_tgt>> /\
+    <<REL2: View.opt_le released2_src released2_tgt>> /\
+    <<STEP1_SRC: Local.read_step lc1_src gl1_src loc ts1 val1 released1_src Ordering.acqrel lc2_src>> /\
+    <<STEP2_SRC: Local.write_step lc2_src gl1_src loc ts1 to2 val2 released1_src released2_src ord2_src lc3_src gl3_src>> /\
+    <<LOCAL3: sim_local lc3_src (local_acquired lc3_tgt)>> /\
+    <<GLOBAL3: sim_global gl3_src gl3_tgt>>.
+Proof.
+  exploit sim_local_read_acquired; eauto. i. des.
+  exploit Local.read_step_future; try exact STEP1_TGT; eauto. i. des.
+  exploit Local.read_step_future; try exact STEP_SRC; eauto. i. des.
+  exploit sim_local_write_acquired; try exact STEP2_TGT; try exact LOCAL2; eauto.
+  { inv STEP1_TGT. inv STEP_SRC. ss.
+    do 2 (condtac; ss).
+    rewrite View.join_bot_r.
+    repeat apply View.join_le; try apply LOCAL1; try refl.
+    inv REL; ss. apply View.bot_spec.
+  }
+  i. des.
+  esplits; try exact STEP_SRC; try exact STEP_SRC0; eauto.
 Qed.
 
 Lemma sim_local_is_racy_acquired
-      lc1_src mem1_src
-      lc1_tgt mem1_tgt
+      lc1_src gl1_src
+      lc1_tgt gl1_tgt
       loc to
-      (STEP_TGT: Local.is_racy lc1_tgt mem1_tgt loc to Ordering.relaxed)
-      (LOCAL1: sim_local SimPromises.bot lc1_src lc1_tgt)
-      (MEM1: sim_memory mem1_src mem1_tgt)
-      (WF1_SRC: Local.wf lc1_src mem1_src)
-      (WF1_TGT: Local.wf lc1_tgt mem1_tgt)
-      (MEM1_SRC: Memory.closed mem1_src)
-      (MEM1_TGT: Memory.closed mem1_tgt):
-  <<STEP_SRC: Local.is_racy lc1_src mem1_src loc to Ordering.acqrel>>.
+      (STEP_TGT: Local.is_racy lc1_tgt gl1_tgt loc to Ordering.relaxed)
+      (LOCAL1: sim_local lc1_src lc1_tgt)
+      (GLOBAL1: sim_global gl1_src gl1_tgt):
+  <<STEP_SRC: Local.is_racy lc1_src gl1_src loc to Ordering.acqrel>>.
 Proof.
   exploit sim_local_is_racy; try exact STEP_TGT;
-    try exact LOCAL1; try exact MEM1; try refl; eauto. i. des.
-  inv x0. econs; eauto.
+    try exact LOCAL1; try exact GLOBAL1; try refl; eauto. i. des.
+  inv x0; eauto.
 Qed.
 
 Lemma sim_local_racy_read_acquired
-      lc1_src mem1_src
-      lc1_tgt mem1_tgt
+      lc1_src gl1_src
+      lc1_tgt gl1_tgt
       loc to val
-      (STEP_TGT: Local.racy_read_step lc1_tgt mem1_tgt loc to val Ordering.relaxed)
-      (LOCAL1: sim_local SimPromises.bot lc1_src lc1_tgt)
-      (MEM1: sim_memory mem1_src mem1_tgt)
-      (WF1_SRC: Local.wf lc1_src mem1_src)
-      (WF1_TGT: Local.wf lc1_tgt mem1_tgt)
-      (MEM1_SRC: Memory.closed mem1_src)
-      (MEM1_TGT: Memory.closed mem1_tgt):
-  <<STEP_SRC: Local.racy_read_step lc1_src mem1_src loc to val Ordering.acqrel>>.
+      (STEP_TGT: Local.racy_read_step lc1_tgt gl1_tgt loc to val Ordering.relaxed)
+      (LOCAL1: sim_local lc1_src lc1_tgt)
+      (GLOBAL1: sim_global gl1_src gl1_tgt):
+  <<STEP_SRC: Local.racy_read_step lc1_src gl1_src loc to val Ordering.acqrel>>.
 Proof.
   inv STEP_TGT.
   exploit sim_local_is_racy_acquired; eauto.
 Qed.
 
 Lemma sim_local_racy_update_acquired
-      lc1_src mem1_src
-      lc1_tgt mem1_tgt
+      lc1_src gl1_src
+      lc1_tgt gl1_tgt
       loc to ow
-      (STEP_TGT: Local.racy_update_step lc1_tgt mem1_tgt loc to Ordering.relaxed ow)
-      (LOCAL1: sim_local SimPromises.bot lc1_src lc1_tgt)
-      (MEM1: sim_memory mem1_src mem1_tgt)
-      (WF1_SRC: Local.wf lc1_src mem1_src)
-      (WF1_TGT: Local.wf lc1_tgt mem1_tgt)
-      (MEM1_SRC: Memory.closed mem1_src)
-      (MEM1_TGT: Memory.closed mem1_tgt):
-  <<STEP_SRC: Local.racy_update_step lc1_src mem1_src loc to Ordering.acqrel ow>>.
+      (STEP_TGT: Local.racy_update_step lc1_tgt gl1_tgt loc to Ordering.relaxed ow)
+      (LOCAL1: sim_local lc1_src lc1_tgt)
+      (GLOBAL1: sim_global gl1_src gl1_tgt):
+  <<STEP_SRC: Local.racy_update_step lc1_src gl1_src loc to Ordering.acqrel ow>>.
 Proof.
-  exploit sim_local_racy_update; try exact STEP_TGT;
-    try exact LOCAL1; try exact MEM1; try refl; eauto. i. des.
-  inv x0.
-  - econs 1; eauto.
-  - econs 2; eauto.
-  - econs 3; eauto.
-    inv RACE. econs; eauto.
+  inv STEP_TGT; eauto.
+  exploit sim_local_is_racy_acquired; eauto.
 Qed.
